---
author: "Pantelis Sopasakis"
title:  "Ideals generated by polynomials"
date: 2025-08-01
description: "Ideals generated by polynomials"
summary: "Ideals generated by polynomials"
math: true
series: ["Mathematix"]
tags: ["Algebra"]
collapsible: true
---

## Definition

We repeat the definition of a ring ideal: 

<div style="border-style:solid;border-width:1.5px;padding: 10px 15px 0px 10px; margin-bottom: 10px" id="def_polynomial_ideal">
    <p><strong>Definition 1: Polynomial ideal.</strong> 
    Consider a polynomial ring $k[x_1, \ldots, x_n]$, where $k$ is a field or a commutative ring. 
    A set $I \subseteq k[x_1, \ldots, x_n]$ is called an ideal if</p>
    <ol>
        <li>$0\in I$</li>
        <li>If $f,g\in I$, then $f+g\in I$</li>
        <li>If $f\in I$ and $h\in k[x_1, \ldots, x_n]$, then $fh\in I$ and $hf\in I$ </li>
    </ol>
</div>
 
<p>As a mini example consider the set $I\subseteq\R[x]$ given by</p> 
<p>$$I=\{a_p x^p + a_{p+1}x^{p+1}+\ldots + a_{p+m}x^{p+m}, a_{p+i}\in \R, m\in \N, i=1,\ldots, m\}.$$</p>
<p>Clearly, $I$ satisfies the three conditions of the definition.</p>

<p>Another ideal is the set of even polynomials, which can have the form $p=a_0+a_2x^2+a_4x^4+\ldots+a_{2k}x^{2k}$.</p>

<div style="border-style:solid;border-width:1.5px;padding: 10px 15px 0px 10px; margin-bottom: 10px" id="def_ideal_generated_by_polynomials">
    <p><strong>Definition 1: Ideal generated by polynomials.</strong> 
    The ideal generated by the polynomials $f_1, \ldots, f_s\in k[x_1,\ldots, x_n]$ is the set</p> 
    <p>$$\langle f_1, \ldots, f_s\rangle = \left\{\sum_{i=1}^{s}h_i f_i : h_1, \ldots, h_s\in k[x_1, \ldots, x_n]\right\}.$$</p>
</div>

<p>We have the following immediate result</p>

<div style="border-style:solid;border-width:1.5px;padding: 10px 15px 0px 10px; margin-bottom: 10px" id="lemma_is_ideal">
    <p><strong>Lemma 1.</strong> 
    The set $\langle f_1, \ldots, f_s\rangle$ is an ideal.</p>
</div>

<p><strong>Example (trivial ideal).</strong> In $k[x]$, the set $\{0\}$ is an ideal. It is generated by the zero polynomial, i.e., $\langle 0\rangle = \{0\}$.</p>

## Some observations

<p>When dealing with a system of polynomial equations</p> 
<p>$$\begin{aligned}
    f_1(x_1, \ldots, x_n) {}={}& 0,\\
    f_2(x_1, \ldots, x_n) {}={}& 0,\\
    \vdots\;\,{}&\\
    f_s(x_1, \ldots, x_n) {}={}& 0,
\end{aligned}$$</p>
<p>we can obtain a new equations. For example, if we multiply the first by $h_1$, the second by $h_2$, etc and sum up, we get</p>
<p>$$h_1f_1+\ldots+h_sf_s = 0,\tag{2}$$</p>
<p>which means that if $(x_1, \ldots, x_n)$ solves the above equations and  $q\in\langle f_1, \ldots, f_s\rangle$, then $q(x_1, \ldots, x_n)=0$.</p>


## Basis


<div style="border-style:solid;border-width:1.5px;padding: 10px 15px 0px 10px; margin-bottom: 10px" id="def_basis_ideal">
    <p><strong>Definition 2: Basis of ideal.</strong> 
    If $I$ is a polynomial ideal and there exist polynomials $f_1, \ldots, f_s$ such that $I=\langle f_1, \ldots, f_s\rangle$, then we say that it is <em>finitely generated</em> and the set $\{f_1, \ldots, f_s\}$ is called a basis of $I$.</p>
</div>

<em>Next we show that</em>

<div style="border-style:solid;border-width:1.5px;padding: 10px 15px 0px 10px; margin-bottom: 10px" id="def_basis_ideal">
    <p><strong>Proposition 1: Equivalent bases define the same variety.</strong> 
    If $\{f_1, \ldots, f_s\}$ and $\{g_1, \ldots, g_t\}$ are two bases for $I$, then </p>
    <p>$$\mathbf{V}(f_1, \ldots, f_s) = \mathbf{V}(g_1, \ldots, g_t).$$</p>
</div>
<!-- ^61b925 -->

<p><em>Proof.</em> Since $\langle f_1, \ldots, f_s\rangle = \langle g_1, \ldots, g_t\rangle$ every "polynomial combination" of the f's can be written as such a combination of the g's. This means that every one of the f's can be written as a polynomial combination of the g's and vice versa. Now take $x\in \mathbf{V}(f_1, \ldots, f_s)$, i.e., $f_1(x)=0$, $\ldots$, $f_s(x)=0$. We'll show that $\mathbf{V}(g_1, \ldots, g_t)$, i.e., we'll show that $g_j(x)=0$, which is easy. $\Box$</p>

<p>We can show that <a href="../hilbert-basis-theorem">every polynomial ideal is finitely generated</a> (this is closely related to Noetherian rings).</p>

## Exercises

These exercises are from[^1], p35-57. Note that Exercises 3a and 3b can be solved like Exercise 3c (better approach).

> **Exercise 3a.**
> Show that $\langle x+y, x-y\rangle = \langle x, y\rangle$

*Solution.* It is
<p>$$\begin{aligned}
\langle x+y, x-y\rangle {}={}& 
\left\{h_1\cdot (x+y) + h_2 \cdot (x-y); h_1, h_2\in k[x, y]\right\} \\
{}={}& \left\{(h_1 + h_2)x + (h_1-h_2)y; h_1, h_2\in k[x, y]\right\} \\
{}={}& \left\{p_1 \cdot x + p_2\cdot y; p_1, p_2\in k[x, y]\right\}. 
\end{aligned}$$<p>
<p>Here we used the fact that for any polynomials $p_1, p_2$ there are polynomials $h_1, h_2$ st $p_1 = h_1+h_2$ and $p_2 = h_1 - h_2$. Simply take $h_1 = \tfrac{1}{2}p_1 + \tfrac{1}{2}p_2$, and $h_2 = \tfrac{1}{2}p_1 - \tfrac{1}{2}p_2$. $\bullet$ </p>

> **Exercise 3b.**
> Show that $\langle x+xy,y+xy,x^2,y^2\rangle = \langle x, y\rangle$

*Solution.* We have 
<p>$$\begin{aligned}
\langle x+xy,y+xy,x^2,y^2\rangle 
{}={}&
\left\{
\left.\begin{array}{l}
h_1 {\cdot} (x+xy)+h_2{\cdot} (y+xy) 
\\
\quad + h_3 {\cdot} x^2 + h_4{\cdot}y^2
\end{array}\;\right|\;
 {} h_i\in k[x,y]\right\}
\\
{}={}&
\{xp_x + y p_y; p_x, p_y\in k[x, y]\},
\end{aligned}$$</p>
<p>and we need to show that for every $p_x, p_y$ there are $h_1,\ldots, h_4$ such that  $p_x = h_1\cdot(1+y) + yh_2 + xh_3$ and $p_y = xh_1 + (1+x)h_2 +yh_4$. Or,</p>
<p>$$\begin{aligned}
p_x ={}& h_1 + xh_3 + y(h_1+h_2),\\
p_y ={}& h_2 + x(h_1+h_2) + yh_4,
\end{aligned}$$</p>
<p>and we can choose $h_2=-h_1$, $h_3=h_4=0$, so the $p_x=h_1$, and $p_y=h_2$. $\bullet$</p>

> **Exercise 3c.**
> Show that $\langle 2x^2 +3y^2 −11,x^2 −y^2 −3\rangle = \langle x^2-4, y^2-1\rangle$

*Solution.* By Euclidean division of polynomials
$$2x^2 +3y^2 −11 = 2(x^2-4) + 3(y^2-1).$$
and 
$$x^2-y^2 -3 = (x^2-4) - (y^2-1).$$
So, look: we define $f_1=2x^2 +3y^2 −11$, $f_2=x^2-y^2 -3$, $g_1=x^2-4$, $g_2=y^2-1$. We have 
<p>$$\begin{aligned}
f_1 ={}& 2g_1 + 3g_2,
\\
f_2 ={}& g_1 - g_2.
\end{aligned}$$</p>
We can solve the system and get
<p>$$\begin{aligned}
g_1 ={}& \tfrac{1}{5}f_1 + \tfrac{3}{5}f_2,
\\
g_2 ={}& \tfrac{1}{5}f_1 - \tfrac{2}{5}f_2.
\end{aligned}$$<p>


For a more detailed exposition, see <a href="../division-multivariate-polynomials">division of multivariate polynomials</a>.

> **Exercise 6.**
> Show that $$\mathbf{V}(x+xy,y+xy,x^2,y^2)=\mathbf{V}(x, y)$$

*Solution.* This is immediate from Exercise 3b and Proposition 1 above. The thing is that if we can find a simpler basis for an ideal, we can also solve simultaneous polynomial equations easier. $\bullet$


## Ideal of variety

<p>Let $V$ be an affine variety<sup>(<a href="#endnotes">1</a>)</sup>, that is, $V$ is the set of solutions of a set of polynomial equations. We ask what are the polynomial equations that have $V$ as their set of solutions (this is an ideal). We give the following definition.</p>

<div style="border-style:solid;border-width:1.5px;padding: 10px 15px 0px 10px; margin-bottom: 10px" id="def_ideal_of_variety">
    <p><strong>Definition 2: ideal of variety.</strong> 
    Let $V \in F^n$ be an affine variety. The ideal of the variety $V$ is defined as </p>
    <p>$$\mathbf{I}(V)=\{f\in k[x_1, \ldots, x_n]: f(a_1, \ldots, a_n)=0, \forall (a_1, \ldots, a_n)\in V\}.$$ </p>
</div>

<p>It's easy to prove that $\mathbf{I}(V)$ is an ideal.</p>

<div style="border-style:solid;border-width:1.5px;padding: 10px 15px 0px 10px; margin-bottom: 10px" id="prop2">
    <p><strong>Proposition 2: $I(V)$ is an ideal</strong> 
    Let $V$ be an affine variety<sup>(<a href="#endnotes">1</a>)</sup>. Then $\mathbf{I}(V)$ is an ideal.</p>    
</div>


<p><em>Proof.</em> $0\in I(V)$ because $0(a_1, \ldots, a_n)=0$ for all $(a_1, \ldots, a_n)\in V$. If $f_1, f_2\in \mathbf{I}(V)$ then $(f_1+f_2)(a_1, \ldots, a_n) = f_1(a_1, \ldots, a_n) + f_2(a_1, \ldots, a_n) = 0$ for all $(a_1, \ldots, a_n)\in V$, so $f_1+f_2\in \mathbf{I}(V)$. Lastly, if $f\in \mathbf{I}(V)$ and $h\in k[x_1, \ldots, x_n]$, then $h(a_1, \ldots, a_n)f(a_1, \ldots, a_n) = 0$ because $f(a_1, \ldots, a_n)=0$ for all $(a_1, \ldots, a_n)\in V$. $\Box$</p>

<p><strong>Example (Ideal of a simple variety).</strong> Consider the variety $V = \{(0, 0)\}$ in $\R^2$. This is the variety of the polynomials $p_1 = x$ and $p_2=y$. In this case, it turns out that the ideal of $V$ is the ideal generated by $p_1$ and $p_2$ (not always true). We will show that </p>
<p>$$\mathbf{I}(V) = \langle x, y\rangle.$$</p>
<p>Take $f\in \langle x, y\rangle$. This means that $f=a(x, y)x + b(x, y)y$. Then $f(0, 0)=0$, i.e., $f$ is zero on $V$, i.e., $f\in \mathbf{I}(V)$. Therefore, $\langle x, y\rangle \subseteq \mathbf{I}(V)$. For the converse, suppose $f\in \mathbf{I}(V)$ and say $f$ has the general form </p>
<p>$$f = a_{0,0} + \sum_{i,j\neq0, 0}a_{i, j}x^i y^j.$$</p>
<p>Since $f(0, 0)=0$, it follows $a_{0, 0}=0$, so </p>
<p>$$f = x\underbrace{\sum_{i>0, j}a_{i, j}x^{i-1} y^j}_{a(x, y)} + y \underbrace{\sum_{i,j>0}a_{i, j}x^i y^{j-1}}_{b(x, y)},$$</p>
<p>which means that $f\in \langle x, y\rangle$. $\bullet$</p>

> **Warning:**
> It is generally not true that $\mathbf{I}(\mathbf{V}(f_1, \ldots, f_s)) = \langle f_1, \ldots, f_s\rangle.$

<p>However, we can prove the following inclusion</p>

<div style="border-style:solid;border-width:1.5px;padding: 10px 15px 0px 10px; margin-bottom: 10px" id="prop3">
    <p><strong>Proposition 3.</strong> 
    We have $\langle f_1, \ldots, f_s\rangle \subseteq \mathbf{I}(\mathbf{V}(f_1, \ldots, f_s))$.
    </p>    
</div>

<p>The proof goes like the first part of the previous example.</p>

<p><strong>Counterexample.</strong> We will show that</p> 
<p>$$\langle x^2, y^2\rangle \subsetneq \mathbf{I}(\mathbf{V}(x^2, y^2)),$$</p>
<p>where</p>
<p>$$\mathbf{V}(x^2, y^2) = \{(x, y): x^2=0, y^2=0\} = \{(0, 0)\},$$</p>
<p>so $\mathbf{I}(\mathbf{V}(x^2, y^2)) = I(\{0, 0\}) = \langle x, y\rangle$ as we saw in the previous example. It is clear that $x\neq \langle x^2, y^2\rangle$. $\bullet$</p>

 
<div style="border-style:dashed;border-width:1.5px;padding: 10px 15px 0px 10px; margin-bottom: 10px" id="note_cox">
    <p><strong>Note.</strong> 
    Cox et al.<sup>[<a href="#references">1</a>]</sup> say that "<em>the ideal of a variety always contains enough information to determine the variety uniquely" and "there is a rich relationship between ideals and affine varieties.</em>"
    </p>    
</div>

<p>The following result is very important:</p>

<div style="border-style:solid;border-width:1.5px;padding: 10px 15px 0px 10px; margin-bottom: 10px" id="prop4">
    <p><strong>Proposition 4: identification of varieties by their ideals.</strong> 
    For two affine varieties $V$ and $W$ in $k^n$,
    </p>    
    <ol>
        <li>$V\subseteq W \iff \mathbf{I}(V) \supseteq \mathbf{I}(W)$</li>
        <li>$V = W \iff \mathbf{I}(V) = \mathbf{I}(W)$</li>
    </ol>
</div>
<!-- ^52dc58 -->

<p><em>Proof.</em> (1) We have</p> 
<p>$$\begin{aligned}
\mathbf{I}(V)={}&\{f\in k[x_1, \ldots, x_n]: f(a_1, \ldots, a_n)=0, \forall (a_1, \ldots, a_n)\in V\}
\\
={}& \bigcap_{(a_1, \ldots, a_n)\in V} \{f\in k[x_1, \ldots, x_n]: f(a_1, \ldots, a_n)=0\},
\end{aligned}$$</p>
<p>from which it is clear that $V\subseteq W$ implies $\mathbf{I}(V) \supseteq \mathbf{I}(W)$. For the converse, assume $\mathbf{I}(V) \supseteq \mathbf{I}(W)$, and $W$ is the set of points $x\in k^n$ such that $g_1(x)=0,\ldots, g_s(x)=0$. Then, $g_1, \ldots, g_s\in \mathbf{I}(W) \subseteq \mathbf{I}(V)$, so the $g_i$ vanish on $V$. In other words, $V$ is an affine variety defined by these $g_i$ and possibly additional polynomials, so $V \subseteq W$.</p>

<p>(2) This is a consequence of (1): $V = W$ means $V \subseteq W$ and $W \subseteq V$; then we apply (1) to show that $\mathbf{I}(V) \supseteq \mathbf{I}(W)$ and $\mathbf{I}(W) \supseteq \mathbf{I}(V)$, so $\mathbf{I}(V) = \mathbf{I}(W)$. $\Box$ </p>

<div style="border-style:solid;border-width:1.5px;padding: 10px 15px 0px 10px; margin-bottom: 10px" id="cor5">
    <p><strong>Corollary 5.</strong> 
    If $V$ and $W$ are affine varieties in $k^n$, then 
    </p>  
    <p>$$V\subsetneq W \iff \mathbf{I}(V) \supsetneq \mathbf{I}(W).$$ </p>
</div>

<p><em>Proof.</em> Immediate from Proposition 4.</p> 


## Univariate polynomials and ideals

<p>Things are particularly simpler in the case of univariate polynomials over a field. There, all ideals are generated by a single element<sup>[<a href="#references">2</a>]</sup>. Such ideals are called <em>principal</em>.</p>

<div style="border-style:solid;border-width:1.5px;padding: 10px 15px 0px 10px; margin-bottom: 10px" id="prop6">
    <p><strong>Proposition 6: all ideals are principal.</strong> 
    Let $k$ be a field. All ideals of $k[x]$ are principal, i.e., for every ideal $I$ there is an $f\in k[x]$ such that $I = \langle f\rangle$.</p>  
</div>
<!-- ^6101ad -->

<p><em>Proof.</em> If $I$ is trivial, i.e., $I=\{0\}$ we know that $I=\langle 0\rangle$, so let us assume that $I$ is nontrivial, i.e., it contains a nonzero polynomial, $f$, of <em>least degree</em>. We will show that $I = \langle f\rangle$. </p>

<p>Since $f\in I$, it follows that $\langle f\rangle \subseteq I$. We need to show that every $g\in I$ can be written as $g=hf$. By the division algorithm, we can write</p>
<p>$$g = qf + r,$$</p>
<p>where $r=0$, or $\deg r < \deg f$. Since $I$ is an ideal and $f\in I$, $qf\in I$. Therefore, $r = g - qf\in I$. If $r\neq 0$ this would mean that we have found a polynomial $r\in I$ with degree less than the degree of $f$. But we assumed that $f$ is polynomial of <em>least degree</em>. This would be a contradiction, so $r=0$. This means that $g = qf$, so $g\in \langle f\rangle$, and $I = \langle f\rangle$. </p>


<div style="border-style:solid;border-width:1.5px;padding: 10px 15px 0px 10px; margin-bottom: 10px" id="prop7">
    <p><strong>Proposition 7: uniqueness of the generator up to scalar multiplication.</strong> 
    Let $k$ be a field. Let $I = \langle f\rangle$ be an ideal of $k[x]$. If there is a function $h$ such that $I = \langle h\rangle$ then $h = \alpha f$, where $\alpha \in k[x]$.</p>  
</div>



## References

1. David A. Cox, John Little, Donal O'Shea, Ideals, Varieties and Algorithms: An Introduction to Computational Algebraic Geometry and Commutative Algebra, Springer, 2015
2. TheoremDep, [Every ideal of a univariate polynomial ring is principal](https://sharmaeklavya2.github.io/theoremdep/nodes/polynomials/every-ideal-is-principal.html), accessed on 3 July 2024


## Endnotes

<ol>
<li>Let $F$ be a field and $p_1,\ldots, p_s\in F[x_1,\ldots, x_n]$ be multivariate polynomials on $F$. The affine variety of $p_1,\ldots, p_s$ is the set $$\mathbf{V}(p_1,\ldots, p_s) = \{(a_1,\ldots, a_n)\in F^n: p_i(a_1,\ldots, a_n)=0, \forall i\}$$ </li>
</ol>